cleanups, split progress into a separate file

theories/contexts.v
@@ -989,6 +989,171 @@ Proof.
     by do 7 eexists; eauto.
 Qed.
 
+Definition ctx_to_cfg (cfg: cfg_tuple_ctx) : option config_tuple :=
+  match cfg with
+  | (s, ccs, sc, oe) =>
+      match rev ccs with
+      | nil => None
+      | (Build_frame_ctx fvs fk ff fes, lcs) :: ccs' =>
+          Some (s, (ff, lcs ⦃ (rev ccs') ⦃ sc ⦃ olist oe ⦄ ⦄ ⦄))
+      end
+  end.
+
+Definition ctx_cfg_typing (cfg: cfg_tuple_ctx) (ts: result_type) : Prop :=
+  match ctx_to_cfg cfg with
+  | Some (s, th) =>
+      config_typing s th ts
+  | None => False
+  end.
+
+Lemma config_typing_inv: forall s (f: frame) es ts,
+    config_typing s (f, es) ts ->
+    exists C,
+      store_typing s /\
+      frame_typing s f C /\
+      e_typing s C es (Tf [::] ts).
+Proof.
+  move => s f es ts Htype; subst.
+  destruct Htype as [Hstoretype Hthtype].
+  inversion Hthtype as [s' f' es' ors rs C' Hstype Hftype ? Hetype]; subst; clear Hthtype.
+  replace (upd_return C' None) with C' in Hetype; first by exists C'.
+  unfold frame_typing in Hftype.
+  remove_bools_options.
+  destruct Hftype as [ts' [-> Hvaltype]] => /=.
+  by unfold inst_typing in Hoption; destruct f, f_inst, t; unfold upd_return, upd_local, upd_local_label_return in *; simpl in *; remove_bools_options.
+Qed.
+
+(* Context typing inversion lemma. The first version preserves the original
+   type label context, where as the second version focuses on the innermost label. *)
+Lemma ctx_cfg_inv_lcs: forall s cc ccs sc oe ts,
+    ctx_cfg_typing (s, (cc :: ccs), sc, oe) ts ->
+    exists C (ret: option result_type) ts2,
+      store_typing s /\
+      frame_typing s cc.1.(FC_frame) C /\
+      (ccs != nil -> (ret = Some ts2 /\ (option_map (@length _) ret = Some cc.1.(FC_arity)))) /\
+      (ccs = nil -> ret = None) /\
+      e_typing s (upd_return C ret) (cc.2 ⦃ sc ⦃ olist oe ⦄ ⦄) (Tf nil ts2).
+Proof.
+  move => s cc ccs sc oe ts Htype.
+  unfold ctx_cfg_typing in Htype.
+  destruct (ctx_to_cfg (s, cc::ccs, sc, oe)) as [[s0 [f es]]|] eqn:Hcfg => //; unfold ctx_to_cfg in Hcfg.
+  destruct (rev (cc :: ccs)) as [ | [[? ? ff ?] lcs] ccs'] eqn:Hcc => //.
+  injection Hcfg as <- <- <-.
+  apply config_typing_inv in Htype as [C [Hstype [Hftype Hetype]]].
+  destruct ccs' using last_ind.
+  + destruct ccs; simpl in * => //; last by apply (f_equal size) in Hcc; rewrite size_rev in Hcc.
+    rewrite rev_cons in Hcc; simpl in *.
+    injection Hcc as -> => /=.
+    exists C, None, ts => /=.
+    repeat split => //.
+    Search frame_typing tc_return.
+    by erewrite <- frame_typing_return_None; eauto; destruct C.
+  + clear IHccs'.
+    rewrite rev_rcons in Hetype.
+    apply lcs_typing_exists in Hetype as [labs0 [ts1 [ts2 [Hetype [Hagree0 Hconsume0]]]]].
+    rewrite rev_cons -rcons_cons in Hcc.
+    apply rcons_inj in Hcc.
+    injection Hcc as Hcc <-.
+    simpl in Hetype.
+    apply rev_move in Hcc; subst.
+    apply ccs_typing_focus in Hetype as [C' [ret [labs [[ts1' ts2'] Hetype]]]].
+    destruct cc as [fc lcs']; simpl in *.
+    invert_e_typing.
+    inversion Hconjl0; subst; clear Hconjl0.
+    exists C0, (Some extr), extr.
+    repeat split => //=; last by move => Hreveq => //=; apply (f_equal size) in Hreveq; rewrite size_rev in Hreveq.
+    by rewrite Hconjr0.
+Qed.
+
+Lemma ctx_cfg_inv: forall s cc ccs sc oe ts,
+    ctx_cfg_typing (s, (cc :: ccs), sc, oe) ts ->
+    exists C (ret: option result_type) labs ts2,
+      store_typing s /\
+      frame_typing s cc.1.(FC_frame) C /\
+      all2 lab_lc_agree labs cc.2 /\ 
+      (ccs != nil -> (option_map (@length _) ret = Some cc.1.(FC_arity))) /\
+      (ccs = nil -> ret = None) /\
+      e_typing s (upd_label (upd_return C ret) labs) (sc ⦃ olist oe ⦄) (Tf nil ts2).
+Proof.
+  move => s cc ccs sc oe ts Htype.
+  apply ctx_cfg_inv_lcs in Htype as [C [ret [ts' [Hstype [Hftype [Hretcons [Hretnil Hetype]]]]]]].
+  apply lcs_typing_exists_nil in Hetype as [labs0 [ts2 [Hetype Hagree0]]].
+  exists C, ret, labs0, ts2.
+  repeat split => //.
+  - move => H; by apply Hretcons in H as [??].
+  - uapply Hetype => /=.
+    f_equal.
+    by erewrite frame_typing_label_empty, cats0; eauto.
+Qed.
+
 End Typing.
+
+Section Reduction.
+
+(** Auxiliary definition for reductions between context tuples. **)
+Definition reduce_ctx (hs hs': host_state) (cfg cfg': cfg_tuple_ctx) : Prop :=
+  match ctx_to_cfg cfg with
+  | Some (s, (f, es)) =>
+      match ctx_to_cfg cfg' with
+      | Some (s', (f', es')) =>
+          reduce hs s f es hs' s' f' es'
+      | None => False
+      end
+  | None => False
+  end.
+
+(** ctx reduction lemmas **)
+(* ctxs reduction can be focused in any partial initial fragments with a pivot cc. *)
+Lemma reduce_focus_pivot ccs0 ccs1: forall hs hs' s ccs sc oe s' sc' oe' cc0 cc0',
+    cc0.1.(FC_val) = cc0'.1.(FC_val) ->
+    cc0.1.(FC_post) = cc0'.1.(FC_post) ->
+    cc0.1.(FC_arity) = cc0'.1.(FC_arity) ->
+    reduce hs s cc0.1.(FC_frame) (cc0.2 ⦃ ccs0 ⦃ sc ⦃ olist oe ⦄ ⦄ ⦄) hs' s' cc0'.1.(FC_frame) (cc0'.2 ⦃ ccs1 ⦃ sc' ⦃ olist oe' ⦄ ⦄ ⦄) ->
+    reduce_ctx hs hs' (s, ccs0 ++ cc0 :: ccs, sc, oe) (s', ccs1 ++ cc0' :: ccs, sc', oe').
+Proof.
+  destruct ccs as [|ccs' cc] using last_ind.
+  - intros ????? [fc lcs] [fc' lcs'] ??? Hred => /=.
+    unfold reduce_ctx, ctx_to_cfg => /=.
+    destruct fc, fc'; simpl in *.
+    do 2 rewrite rev_cat /= revK.
+    exact Hred.
+  - intros ????? [fc lcs] [fc' lcs'] Heqval Heqpost Heqarity Hred.
+    unfold reduce_ctx, ctx_to_cfg in * => /=.
+    destruct cc as [[fvs0 fk0 ff0 fes0] lcs0].
+    rewrite rev_cat rev_cons rev_rcons /=.
+    repeat rewrite rev_cat rev_rcons revK.
+    rewrite rev_cat rev_cons rev_rcons revK /= rev_cat rev_rcons revK revK.
+    apply (list_label_ctx_eval.(ctx_reduce)) => //.
+    do 2 rewrite foldl_cat.
+    simpl in *.
+    apply (list_closure_ctx_eval.(ctx_reduce)) => //.
+    rewrite -Heqval -Heqpost -Heqarity.
+    eapply r_label with (lh := LH_base (rev (FC_val fc)) (FC_post fc)) => /=; try by (f_equal; rewrite -cat1s; eauto).
+    by apply r_frame.
+Qed.
+
+Lemma reduce_focus: forall ccs hs s lcs sc oe hs' s' lcs' sc' oe' fc fc',
+    fc.(FC_val) = fc'.(FC_val) ->
+    fc.(FC_post) = fc'.(FC_post) ->
+    fc.(FC_arity) = fc'.(FC_arity) ->
+    reduce hs s fc.(FC_frame) (lcs ⦃ sc ⦃ olist oe ⦄ ⦄) hs' s' fc'.(FC_frame) (lcs' ⦃ sc' ⦃ olist oe' ⦄ ⦄) ->
+    reduce_ctx hs hs' (s, (fc, lcs) :: ccs, sc, oe) (s', (fc', lcs') :: ccs, sc', oe').
+Proof.
+  intros; by apply (@reduce_focus_pivot nil nil).
+Qed.
+
+Lemma reduce_focus_id: forall ccs hs s lcs sc oe hs' s' sc' oe' fc fc',
+    fc.(FC_val) = fc'.(FC_val) ->
+    fc.(FC_post) = fc'.(FC_post) ->
+    fc.(FC_arity) = fc'.(FC_arity) ->
+    reduce hs s fc.(FC_frame) (sc ⦃ olist oe ⦄) hs' s' fc'.(FC_frame) (sc' ⦃ olist oe' ⦄) ->
+    reduce_ctx hs hs' (s, (fc, lcs) :: ccs, sc, oe) (s', (fc', lcs) :: ccs, sc', oe').
+Proof.
+  intros ???????????? Heqval Heqpost Heqarity Hred => /=.
+  apply reduce_focus => //.
+  by apply (list_label_ctx_eval.(ctx_reduce)) with (hs := hs) => //.
+Qed.
+
+End Reduction.
 
 End Host.
