theories/interpreter_ctx.v
@@ -15,188 +15,10 @@ Section Host.
 
 Context `{ho: host}.
   
-Variable host_application_impl : host_state -> store_record -> function_type -> host_function -> seq value ->
-                       (host_state * option (store_record * result)).
+Variable host_application_impl : host_state -> store_record -> function_type -> host_function -> seq value -> (host_state * option (store_record * result)).
 
 Hypothesis host_application_impl_correct :
   (forall hs s ft hf vs hs' hres, (host_application_impl hs s ft hf vs = (hs', hres)) -> host_application hs s ft hf vs hs' hres).
-
-Notation "ctx ⦃ es ⦄" := (ctx_fill es ctx) (at level 1).
-
-Definition ctx_to_cfg (cfg: cfg_tuple_ctx) : option config_tuple :=
-  match cfg with
-  | (s, ccs, sc, oe) =>
-      match rev ccs with
-      | nil => None
-      | (Build_frame_ctx fvs fk ff fes, lcs) :: ccs' =>
-          Some (s, (ff, lcs ⦃ (rev ccs') ⦃ sc ⦃ olist oe ⦄ ⦄ ⦄))
-      end
-  end.
-
-Definition ctx_cfg_typing (cfg: cfg_tuple_ctx) (ts: result_type) : Prop :=
-  match ctx_to_cfg cfg with
-  | Some (s, th) =>
-      config_typing s th ts
-  | None => False
-  end.
-
-Lemma config_typing_inv: forall s (f: frame) es ts,
-    config_typing s (f, es) ts ->
-    exists C,
-      store_typing s /\
-      frame_typing s f C /\
-      e_typing s C es (Tf [::] ts).
-Proof.
-  move => s f es ts Htype; subst.
-  destruct Htype as [Hstoretype Hthtype].
-  inversion Hthtype as [s' f' es' ors rs C' Hstype Hftype ? Hetype]; subst; clear Hthtype.
-  replace (upd_return C' None) with C' in Hetype; first by exists C'.
-  unfold frame_typing in Hftype.
-  remove_bools_options.
-  destruct Hftype as [ts' [-> Hvaltype]] => /=.
-  by unfold inst_typing in Hoption; destruct f, f_inst, t; unfold upd_return, upd_local, upd_local_label_return in *; simpl in *; remove_bools_options.
-Qed.
-
-(* Context typing inversion lemma. The first version preserves the original
-   type label context, where as the second version focuses on the innermost label. *)
-Lemma ctx_cfg_inv_lcs: forall s cc ccs sc oe ts,
-    ctx_cfg_typing (s, (cc :: ccs), sc, oe) ts ->
-    exists C (ret: option result_type) ts2,
-      store_typing s /\
-      frame_typing s cc.1.(FC_frame) C /\
-      (ccs != nil -> (ret = Some ts2 /\ (option_map (@length _) ret = Some cc.1.(FC_arity)))) /\
-      (ccs = nil -> ret = None) /\
-      e_typing s (upd_return C ret) (cc.2 ⦃ sc ⦃ olist oe ⦄ ⦄) (Tf nil ts2).
-Proof.
-  move => s cc ccs sc oe ts Htype.
-  unfold ctx_cfg_typing in Htype.
-  destruct (ctx_to_cfg (s, cc::ccs, sc, oe)) as [[s0 [f es]]|] eqn:Hcfg => //; unfold ctx_to_cfg in Hcfg.
-  destruct (rev (cc :: ccs)) as [ | [[? ? ff ?] lcs] ccs'] eqn:Hcc => //.
-  injection Hcfg as <- <- <-.
-  apply config_typing_inv in Htype as [C [Hstype [Hftype Hetype]]].
-  destruct ccs' using last_ind.
-  + destruct ccs; simpl in * => //; last by apply (f_equal size) in Hcc; rewrite size_rev in Hcc.
-    rewrite rev_cons in Hcc; simpl in *.
-    injection Hcc as -> => /=.
-    exists C, None, ts => /=.
-    repeat split => //.
-    Search frame_typing tc_return.
-    by erewrite <- frame_typing_return_None; eauto; destruct C.
-  + clear IHccs'.
-    rewrite rev_rcons in Hetype.
-    apply lcs_typing_exists in Hetype as [labs0 [ts1 [ts2 [Hetype [Hagree0 Hconsume0]]]]].
-    rewrite rev_cons -rcons_cons in Hcc.
-    apply rcons_inj in Hcc.
-    injection Hcc as Hcc <-.
-    simpl in Hetype.
-    apply rev_move in Hcc; subst.
-    apply ccs_typing_focus in Hetype as [C' [ret [labs [[ts1' ts2'] Hetype]]]].
-    destruct cc as [fc lcs']; simpl in *.
-    invert_e_typing.
-    inversion Hconjl0; subst; clear Hconjl0.
-    exists C0, (Some extr), extr.
-    repeat split => //=; last by move => Hreveq => //=; apply (f_equal size) in Hreveq; rewrite size_rev in Hreveq.
-    by rewrite Hconjr0.
-Qed.
-
-Lemma ctx_cfg_inv: forall s cc ccs sc oe ts,
-    ctx_cfg_typing (s, (cc :: ccs), sc, oe) ts ->
-    exists C (ret: option result_type) labs ts2,
-      store_typing s /\
-      frame_typing s cc.1.(FC_frame) C /\
-      all2 lab_lc_agree labs cc.2 /\ 
-      (ccs != nil -> (option_map (@length _) ret = Some cc.1.(FC_arity))) /\
-      (ccs = nil -> ret = None) /\
-      e_typing s (upd_label (upd_return C ret) labs) (sc ⦃ olist oe ⦄) (Tf nil ts2).
-Proof.
-  move => s cc ccs sc oe ts Htype.
-  apply ctx_cfg_inv_lcs in Htype as [C [ret [ts' [Hstype [Hftype [Hretcons [Hretnil Hetype]]]]]]].
-  apply lcs_typing_exists_nil in Hetype as [labs0 [ts2 [Hetype Hagree0]]].
-  exists C, ret, labs0, ts2.
-  repeat split => //.
-  - move => H; by apply Hretcons in H as [??].
-  - uapply Hetype => /=.
-    f_equal.
-    by erewrite frame_typing_label_empty, cats0; eauto.
-Qed.
-
-(** Auxiliary definition for reductions between context tuples. **)
-Definition reduce_ctx (hs hs': host_state) (cfg cfg': cfg_tuple_ctx) : Prop :=
-  match ctx_to_cfg cfg with
-  | Some (s, (f, es)) =>
-      match ctx_to_cfg cfg' with
-      | Some (s', (f', es')) =>
-          reduce hs s f es hs' s' f' es'
-      | None => False
-      end
-  | None => False
-  end.
-
-(** ctx reduction lemmas **)
-(* ctxs reduction can be focused in any partial initial fragments with a pivot cc. *)
-Lemma reduce_focus_pivot ccs0 ccs1: forall hs hs' s ccs sc oe s' sc' oe' cc0 cc0',
-    cc0.1.(FC_val) = cc0'.1.(FC_val) ->
-    cc0.1.(FC_post) = cc0'.1.(FC_post) ->
-    cc0.1.(FC_arity) = cc0'.1.(FC_arity) ->
-    reduce hs s cc0.1.(FC_frame) (cc0.2 ⦃ ccs0 ⦃ sc ⦃ olist oe ⦄ ⦄ ⦄) hs' s' cc0'.1.(FC_frame) (cc0'.2 ⦃ ccs1 ⦃ sc' ⦃ olist oe' ⦄ ⦄ ⦄) ->
-    reduce_ctx hs hs' (s, ccs0 ++ cc0 :: ccs, sc, oe) (s', ccs1 ++ cc0' :: ccs, sc', oe').
-Proof.
-  destruct ccs as [|ccs' cc] using last_ind.
-  - intros ????? [fc lcs] [fc' lcs'] ??? Hred => /=.
-    unfold reduce_ctx, ctx_to_cfg => /=.
-    destruct fc, fc'; simpl in *.
-    do 2 rewrite rev_cat /= revK.
-    exact Hred.
-  - intros ????? [fc lcs] [fc' lcs'] Heqval Heqpost Heqarity Hred.
-    unfold reduce_ctx, ctx_to_cfg in * => /=.
-    destruct cc as [[fvs0 fk0 ff0 fes0] lcs0].
-    rewrite rev_cat rev_cons rev_rcons /=.
-    repeat rewrite rev_cat rev_rcons revK.
-    rewrite rev_cat rev_cons rev_rcons revK /= rev_cat rev_rcons revK revK.
-    apply (list_label_ctx_eval.(ctx_reduce)) => //.
-    do 2 rewrite foldl_cat.
-    simpl in *.
-    apply (list_closure_ctx_eval.(ctx_reduce)) => //.
-    rewrite -Heqval -Heqpost -Heqarity.
-    eapply r_label with (lh := LH_base (rev (FC_val fc)) (FC_post fc)) => /=; try by (f_equal; rewrite -cat1s; eauto).
-    by apply r_frame.
-Qed.
-
-Lemma reduce_focus: forall ccs hs s lcs sc oe hs' s' lcs' sc' oe' fc fc',
-    fc.(FC_val) = fc'.(FC_val) ->
-    fc.(FC_post) = fc'.(FC_post) ->
-    fc.(FC_arity) = fc'.(FC_arity) ->
-    reduce hs s fc.(FC_frame) (lcs ⦃ sc ⦃ olist oe ⦄ ⦄) hs' s' fc'.(FC_frame) (lcs' ⦃ sc' ⦃ olist oe' ⦄ ⦄) ->
-    reduce_ctx hs hs' (s, (fc, lcs) :: ccs, sc, oe) (s', (fc', lcs') :: ccs, sc', oe').
-Proof.
-  intros; by apply (@reduce_focus_pivot nil nil).
-Qed.
-
-Lemma reduce_focus_id: forall ccs hs s lcs sc oe hs' s' sc' oe' fc fc',
-    fc.(FC_val) = fc'.(FC_val) ->
-    fc.(FC_post) = fc'.(FC_post) ->
-    fc.(FC_arity) = fc'.(FC_arity) ->
-    reduce hs s fc.(FC_frame) (sc ⦃ olist oe ⦄) hs' s' fc'.(FC_frame) (sc' ⦃ olist oe' ⦄) ->
-    reduce_ctx hs hs' (s, (fc, lcs) :: ccs, sc, oe) (s', (fc', lcs) :: ccs, sc', oe').
-Proof.
-  intros ???????????? Heqval Heqpost Heqarity Hred => /=.
-  apply reduce_focus => //.
-  by apply (list_label_ctx_eval.(ctx_reduce)) with (hs := hs) => //.
-Qed.
-
-Ltac red_ctx_simpl :=
-  repeat lazymatch goal with
-  | |- reduce _ _ _ (((_, ?lcs) :: ?ccs) ⦃ _ ⦃ _ ⦄ ⦄) _ _ _ (((_, ?lcs) :: ?ccs) ⦃ _ ⦃ _ ⦄ ⦄) =>
-      apply reduce_focus_id
-  | |- reduce _ _ _ (((_, _) :: ?ccs) ⦃ _ ⦃ _ ⦄ ⦄) _ _ _ (((_, _) :: ?ccs) ⦃ _ ⦃ _ ⦄ ⦄) =>
-      apply reduce_focus
-  | |- reduce _ _ _ (?ccs ⦃ _ ⦃ _ ⦄ ⦄) _ _ _ (?ccs ⦃ _ ⦃ _ ⦄ ⦄) =>
-      apply (list_closure_ctx_eval.(ctx_reduce))
-  | |- reduce _ _ _ (foldl closure_ctx_fill _ _) _ _ _ (foldl closure_ctx_fill _ _) =>
-      apply (list_closure_ctx_eval.(ctx_reduce))
-  | |- reduce _ _ _ (foldl label_ctx_fill _ _) _ _ _ (foldl label_ctx_fill _ _) =>
-      apply (list_label_ctx_eval.(ctx_reduce))
-  end.
 
 (** Automatically trying to infer what to put aside using the L0 context (r_label) **)
 Ltac infer_hole :=
@@ -237,27 +59,8 @@ Ltac infer_hole :=
       f_equal => //=
   end.
 
-
 Ltac resolve_reduce_ctx vs es :=
   try apply reduce_focus_id => //; try (eapply r_label with (lh := LH_base (rev vs) es) => /=; infer_hole).
-
-Ltac resolve_valid_ccs :=
-  repeat lazymatch goal with
-    | |- _ /\ _ =>
-        split => //
-    | |- context C [valid_ccs _] =>
-        unfold valid_ccs => /=
-    end.
-
-Definition s_of_cfg (cfg: cfg_tuple_ctx) :=
-  match cfg with
-  | (s, _, _, _) => s
-  end.
-
-Definition es_of_cfg (cfg: cfg_tuple_ctx) :=
-  match cfg with
-  | (_, ccs, sc, oe) => ccs ⦃ sc ⦃ olist oe ⦄ ⦄
-  end.
 
 Definition valid_ccs_cfg (cfg: cfg_tuple_ctx) :=
   let '(s, ccs, sc, oe) := cfg in
@@ -443,7 +246,7 @@ Proof.
         (* types are all defaultable as of Wasm 2.0. This potentially needs a 
            small change in 3.0. *)
         { apply <<hs, (s, (Build_frame_ctx vs'' m (Build_frame (rev vs' ++ zs) i) es0, nil) :: (fc, lcs) :: ccs', (nil, nil), Some (AI_label m nil (to_e_list es)))>> => //=.
-          apply (@reduce_focus_pivot nil ([::(Build_frame_ctx vs'' m _ es0, nil)])) => //=.
+          apply (@reduce_focus_pivot _ _ nil ([::(Build_frame_ctx vs'' m _ es0, nil)])) => //=.
           apply (list_label_ctx_eval.(ctx_reduce)) => //=.
           rewrite split_n_is_take_drop in Hsplit; injection Hsplit as <- <-.
           eapply r_label with (lh := LH_base (rev (drop n vs0)) es0) => /=; subst; infer_hole.
@@ -632,6 +435,8 @@ end.
 Ltac discriminate_value_type :=
   resolve_invalid_typing; resolve_invalid_value.
 
+(* Directly destructs the top value of stack and automatically resolve the ill-typed
+   cases. *)
 Ltac assert_value_num v :=
   destruct v as [v | |]; [ | by discriminate_value_type | by discriminate_value_type].
 
@@ -679,7 +484,7 @@ Proof.
             (* Exiting the frame now. Note that this implementation does not 
                attempt to directly construct the next canonical cfg (les can be non-empty) *)
             apply <<hs, (s, cc :: ccs', (vs0 ++ lvs, les), None)>> => //=.
-            apply (@reduce_focus_pivot [:: (Build_frame_ctx lvs lk lf les, nil)] nil) => //=.
+            apply (@reduce_focus_pivot _ _ [:: (Build_frame_ctx lvs lk lf les, nil)] nil) => //=.
             apply (list_label_ctx_eval.(ctx_reduce)) => //=.
             repeat rewrite cats0.
             resolve_reduce_ctx lvs les.
@@ -1827,10 +1632,6 @@ Proof.
     destruct (ctx_decompose_aux _) as [[[??]?]|] eqn:Hdecomp => //; by apply ctx_decompose_acc_some in Hdecomp.
 Defined.
 
-Definition hs_cfg_ctx : Type := host_state * cfg_tuple_ctx.
-
-Definition empty_store_record := Build_store_record nil nil nil nil nil nil.
-
 Fixpoint run_multi_step_ctx (fuel: nat) (hs: host_state) (cfg: cfg_tuple_ctx) : (option unit) + (list value) :=
   match fuel with
   | 0 => inl None
@@ -1854,43 +1655,6 @@ Definition run_multi_step_raw (hs: host_state) (fuel: nat) (s: store_record) (f:
   match run_v_init_with_frame s f es with
   | exist cfg _ => run_multi_step_ctx fuel hs cfg
   end.
-
-Section Interp_ctx_progress.
-
-(* Derive the progress property from the interpreter *)
-Definition t_progress_interp_ctx: forall (hs: host_state) (s: store_record) (f: frame) es ts,
-  config_typing s (f, es) ts ->
-  terminal_form es \/
-    (exists hs' s' f' es', reduce hs s f es hs' s' f' es').
-Proof.
-  move => hs s f es ts Htype.
-  (* initialise an interpreter cfg tuple *)
-  destruct (run_v_init_with_frame s f es) as [[[[s0 ccs] sc] oe] [Hfill Hvalid]].
-  (* run the interpreter *)
-  remember (run_one_step_ctx hs (s0, ccs, sc, oe)) as res.
-  destruct res as [hs' [[[s' ccs'] sc'] oe'] Hred Hvalid' | s' f' vs Hvalfill | s' f' Htrapfill | Hcontra | Hcontra]; clear Heqres.
-  (* step *)
-  - unfold reduce_ctx in Hred.
-    rewrite Hfill in Hred.
-    destruct (ctx_to_cfg (s', ccs', sc', oe')) as [[s'' [f'' es'']] | ] => //.
-    right.
-    by exists hs', s'', f'', es''.
-  (* values *)
-  - rewrite Hvalfill in Hfill; injection Hfill as <- <- <-.
-    do 2 left.
-    by apply v_to_e_const.
-  (* trap *)
-  - rewrite Htrapfill in Hfill; injection Hfill as <- <- <-.
-    by left; right.
-  (* invalid input -- impossible *)
-  - by apply Hcontra in Hvalid.
-  (* ill-typed -- impossible *)
-  - unfold ctx_cfg_typing in Hcontra.
-    rewrite Hfill in Hcontra.
-    by apply Hcontra in Htype.
-Qed.
-
-End Interp_ctx_progress.
 
 End Host.
 
@@ -1932,11 +1696,5 @@ Definition run_step_cfg_ctx_reform : cfg_tuple_ctx -> option cfg_tuple_ctx := ru
 Definition run_v_init : store_record -> list administrative_instruction -> option cfg_tuple_ctx := run_v_init.
 
 Definition run_v_init_with_frame := run_v_init_with_frame.
-
-Definition run_multi_step_raw : host_state -> nat -> store_record -> frame -> list administrative_instruction -> (option unit) + (list value) := run_multi_step_raw host_application_impl_correct.
-
-Definition es_of_cfg : cfg_tuple_ctx -> list administrative_instruction := es_of_cfg.
-
-Definition s_of_cfg : cfg_tuple_ctx -> store_record := s_of_cfg.
 
 End Interpreter_ctx_extract.
