theories/type_progress.v
@@ -1,0 +1,54 @@
+From Wasm Require Export interpreter_ctx.
+From Coq Require Import ZArith.BinInt Program.Equality.
+From mathcomp Require Import ssreflect ssrfun ssrnat ssrbool eqtype seq.
+Require Import BinNat NArith BinNums ZArith.
+
+Set Implicit Arguments.
+Unset Strict Implicit.
+
+Unset Printing Implicit Defensive.
+
+Section Host.
+
+Context `{ho: host}.
+
+(* The same host function well-formedness assumptions from the interpreter *)
+Variable host_application_impl : host_state -> store_record -> function_type -> host_function -> seq value -> (host_state * option (store_record * result)).
+
+Hypothesis host_application_impl_correct :
+  (forall hs s ft hf vs hs' hres, (host_application_impl hs s ft hf vs = (hs', hres)) -> host_application hs s ft hf vs hs' hres).
+
+(* The progress property is derived from the interpreter. *)
+Definition t_progress_interp_ctx: forall (hs: host_state) (s: store_record) (f: frame) es ts,
+  config_typing s (f, es) ts ->
+  terminal_form es \/
+    (exists hs' s' f' es', reduce hs s f es hs' s' f' es').
+Proof.
+  move => hs s f es ts Htype.
+  (* initialise an interpreter cfg tuple *)
+  destruct (run_v_init_with_frame s f es) as [[[[s0 ccs] sc] oe] [Hfill Hvalid]].
+  (* run the interpreter *)
+  remember (@run_one_step_ctx _ _ host_application_impl host_application_impl_correct hs (s0, ccs, sc, oe)) as res.
+  destruct res as [hs' [[[s' ccs'] sc'] oe'] Hred Hvalid' | s' f' vs Hvalfill | s' f' Htrapfill | Hcontra | Hcontra]; clear Heqres.
+  (* step *)
+  - unfold reduce_ctx in Hred.
+    rewrite Hfill in Hred.
+    destruct (ctx_to_cfg (s', ccs', sc', oe')) as [[s'' [f'' es'']] | ] => //.
+    right.
+    by exists hs', s'', f'', es''.
+  (* values *)
+  - rewrite Hvalfill in Hfill; injection Hfill as <- <- <-.
+    do 2 left.
+    by apply v_to_e_const.
+  (* trap *)
+  - rewrite Htrapfill in Hfill; injection Hfill as <- <- <-.
+    by left; right.
+  (* invalid input -- impossible *)
+  - by apply Hcontra in Hvalid.
+  (* ill-typed -- impossible *)
+  - unfold ctx_cfg_typing in Hcontra.
+    rewrite Hfill in Hcontra.
+    by apply Hcontra in Htype.
+Qed.
+
+End Host.
